hax-lib/proof-libs/lean/Hax/Rust_primitives/Boxed.lean
@@ -1,2 +1,2 @@
 
-abbrev alloc.Boxed.Box (T _Allocator : Type) := T
+abbrev alloc.boxed.Box (T _Allocator : Type) := T
