hax-lib/proof-libs/lean/Hax/Rust_primitives/Mem.lean
@@ -1,5 +1,5 @@
 import Hax.Rust_primitives.RustM
 import Hax.Rust_primitives.Tuple
 
-def rust_primitives.Mem.replace (α : Type) (dst : α) (src : α) :
+def rust_primitives.mem.replace (α : Type) (dst : α) (src : α) :
   RustM (rust_primitives.hax.Tuple2 α α) := pure ⟨src, dst⟩
