hax-lib/proof-libs/lean/Hax/Rust_primitives/String.lean
@@ -1,3 +1,3 @@
 
 abbrev string_indirection : Type := String
-abbrev alloc.String.String : Type := string_indirection
+abbrev alloc.string.String : Type := string_indirection
